QF_S.thy
@@ -3,12 +3,16 @@ theory QF_S
 begin
 
 
-abbreviation str_concat:: "'a word \<Rightarrow> 'a word  \<Rightarrow> 'a word"  where "(str_concat) u v \<equiv> u*v" 
-abbreviation str_len:: "'a word \<Rightarrow> nat" where  "str_len w \<equiv> size w"
-abbreviation str_at:: "'a word \<Rightarrow> nat \<Rightarrow> 'a word" where "str_at w i \<equiv> (case (at w i) of (option.Some a) \<Rightarrow> (Con a  Epsilon) | option.None \<Rightarrow> Epsilon)"
+abbreviation str_concat:: "'a word \<Rightarrow> 'a word  \<Rightarrow> 'a word"  where "(str_concat) u v \<equiv> u@v" 
+abbreviation str_len:: "'a word \<Rightarrow> int" where  "str_len w \<equiv> of_nat (length w)"
+abbreviation str_at:: "'a word \<Rightarrow> int \<Rightarrow> 'a word" where "str_at w i \<equiv> (at w (nat i))"
 
+abbreviation str_substr:: "'a word \<Rightarrow> int \<Rightarrow> int \<Rightarrow> 'a word"  where "str_substr a i n \<equiv>  fac a (nat i) (nat n)"
 abbreviation str_prefixof:: "'a word \<Rightarrow> 'a word \<Rightarrow> bool" where "str_prefixof \<equiv> Words.is_prefix"
 abbreviation str_suffixof:: "'a word \<Rightarrow> 'a word \<Rightarrow> bool" where "str_suffixof \<equiv> Words.is_suffix"
+abbreviation str_contains:: "'a word \<Rightarrow> 'a word \<Rightarrow> bool" where "str_contains \<equiv> Words.contains"
+abbreviation str_indexof:: "'a word \<Rightarrow> 'a word \<Rightarrow> int \<Rightarrow> int" 
+  where "str_indexof h n s \<equiv> of_nat (find h n)"
 
 (* Regular Expression Functions *)
 
